steel/Veritas.Steel.Log.fsti
@@ -1,0 +1,116 @@
+module Veritas.Steel.Log
+module T = Veritas.Formats.Types
+module A = Steel.Array
+module U8 = FStar.UInt8
+module U32 = FStar.UInt32
+open Steel.Memory
+open Steel.Effect
+
+let repr = Ghost.erased (Seq.seq T.vlog_entry)
+let empty_log : repr = Seq.empty
+let snoc_log (r:repr) (e:T.vlog_entry) : repr = Seq.snoc r e
+
+(* [log] : The main abstract type of this module
+
+   Internally, it is represented as a quadruple
+     * a: An array of bytes
+     * l: length of the array
+     * p: ref (n:U32.t{n <= l}), a mutable current position in the array,
+     * g: A ghost reference of a sequence of log entries
+*)
+val log : Type0
+
+val log_len (l:log) : U32.t
+
+val log_array (l:log) : A.array U8.t
+
+(* [log_with_parsed_prefix] : The main representation predicate
+
+   Internally, it states:
+     * varray a: Permission on the underlying array
+
+     * vptr p: Permision on the current position
+
+     * vghostpr g: Permission on the ghost ref
+
+     * an invariant stating that the array is validated from 0 to p,
+       and current value of g is parsed prefix of a
+*)
+val log_with_parsed_prefix (l:log) (s:repr) : vprop
+
+(* To create a log, call initialize log with an array of bytes *)
+val initialize_log (len:U32.t) (a:A.array U8.t)
+  : Steel log
+    (A.varray a)
+    (fun l -> log_with_parsed_prefix l empty_log)
+    (requires fun _ -> True)
+    (ensures fun _ l _ ->
+      log_len l == len /\
+      log_array l == a)
+
+(* The main idea of the interface is that one can repeatedly call
+   read_next to try to read the next entry from the log.
+
+   When the log is fully read, we return a **pure predicate**
+   [parsed_log l s] which witnesses that the content of the log was
+   exactly s.
+*)
+
+(*
+  [parsed_log_inv i l n s]: This is implemented as a Steel invariant.
+
+      i >--> parsed_log l s n
+
+  where parsed_log l n s : slprop =
+        pure (Seq.length s = n) `star` l.g `pts_to` s
+
+  i.e., that the ghost ref of l points to the sequence
+
+  Because I need this invariant, I'm using indexed slprops
+  rather than selectors
+*)
+val parsed_log_inv (i:iname)
+                   (l:log)
+                   (n:U32.t)
+                   (s:repr)
+  : prop
+
+(* [read_result]: Three potential results from trying to read an entry *)
+noeq
+type read_result =
+  | Finished of iname
+  | Parsed_with_maybe_more of T.vlog_entry
+  | Failed:  pos:U32.t -> msg:string -> read_result
+
+(* [read_next]:
+    - To call [read_next], the caller needs to own the `log_with_parsed_prefix` permission
+    - In return, there are three cases
+
+      * If the log is finished, we return an invariant showing that
+        the log contained s and return back permission on the
+        underyling array to the caller. Internally, we will also
+        deallocate any other state, notably the pointer to the current
+        position
+
+      * If we successfully parse another entry, we return it,
+        extending the parsed prefix.
+
+      * If parsing fails, we deallocate our internal state, return
+        permission to the underlying array, and signal back a position
+        at which parsing failed and an error message.
+*)
+val read_next (#s:repr)
+              (l:log)
+  : Steel read_result
+    (log_with_parsed_prefix l s)
+    (fun o ->
+      match o with
+      | Finished i -> A.varray (log_array l)
+      | Parsed_with_maybe_more e -> log_with_parsed_prefix l (snoc_log s e)
+      | Failed pos _ -> A.varray (log_array l))
+    (requires fun _ -> True)
+    (ensures fun _ o _ ->
+      match o with
+      | Finished i -> parsed_log_inv i l (log_len l) s
+      | Parsed_with_maybe_more e -> True
+      | Failed pos _ -> U32.(pos <^ log_len l))
